icon:: ðŸŸ¦
inherit-color-icon-from:: [[logseq-page-color-blue]] 
template-used:: standard-page
tags:: [[wellensausbreitung]], [[uni]]
alias:: hew

- $+ \cfrac{\partial}{\partial z}e_{y} = \mu \cfrac{\partial}{\partial t}h_{x}$
- $- \cfrac{\partial}{\partial z}e_{x} = \mu \cfrac{\partial}{\partial t}h_{y}$
- $0 = \mu \cfrac{\partial}{\partial t}h_{z}$
- $- \cfrac{\partial}{\partial z}h_{y} = \varepsilon \cfrac{\partial}{\partial t}e_{x}$
- $+ \cfrac{\partial}{\partial z}h_{x} = \varepsilon \cfrac{\partial}{\partial t}e_{y}$
- $0 = \varepsilon \cfrac{\partial}{\partial t}e_{z}$
- $\cfrac{\partial^2}{\partial z^2}e_{x} - \mu \varepsilon \cfrac{\partial^2}{\partial t^2}e_{x} = 0$
- $e_{x}\left(z,t\right) = \underbrace{c_1f_1\left(z - vt\right)}_{ = e_{x}^{ + }\left(z,t\right)} + \underbrace{c_2f_2\left(z + vt\right)}_{ = e_{x}^{ - }\left(z,t\right)}$
- $v = \cfrac{1}{\sqrt{\varepsilon \mu}} = \cfrac{\omega}{k}$
- $\eta = \sqrt{\cfrac{\mu}{\varepsilon}}$
- $\eta = \eta_0 = \sqrt{\cfrac{\mu_0}{\varepsilon_0}} \approx120 \pi \Omega \approx377 \Omega$
- $h_{x}^{ + } = - \cfrac{e_{y}^{ + }}{\eta}$
- $\cfrac{e_{x}^{ + }}{h_{y}^{ + }} = - \cfrac{e_{y}^{ + }}{h_{x}^{ + }} = \eta$
- $\vect{E} \perp \vect{H} \perp \vect{i}_{z}$
- $\cfrac{e_{x}^{ - }}{h_{y}^{ - }} = - \cfrac{e_{y}^{ - }}{h_{x}^{ - }} = - \eta$
- $w_{\opn{e}}\left(t\right) = \cfrac{\varepsilon}{2}\left(e_{x}^2 + e_{y}^2\right)$
- $w_{\opn{m}}\left(t\right) = \cfrac{\mu}{2}\left(h_{x}^2 + h_{y}^2\right)$
- $w_{\opn{m}}\left(t\right) = \cfrac{\mu}{2} \cfrac{1}{\eta^2}\left(e_{x}^2 + e_{y}^2\right) = w_{\opn{e}}\left(t\right)$
- ${p_{x}^{+}\equiv0}$
- ${p_{y}^{ + } \equiv 0}$
- ${p_{z}^{+}=e_{x}^{+}h_{y}^{+}}-{e_{y}^{+}h_{x}^{+}}$
- ${p_{z}^{+}=-\cfrac{1}{\eta}\left(e_{r}^{+^2}+e_{y}^{+^2}\right)}$
- $\overline{\vect{P}\left(t\right)}=\overline{\vect{E}\times \vect{H}}=\cfrac{1}{\eta}\left(\overline{{e_{x}^{+}}^2+{e_{y}^{+}}^2}\right)\vect{i}_{z}=\cfrac{1}{2\eta}\left(\overline{E_{x0}^2+E_{y0}^2}\right)\vect{i}_{z}$
- $e_{x}\left(z,t\right) = \operatorname{Re} \{E_{x}\left(z\right)e^{j \omega t} \} = E_0 \cos \left(k\left(vt - z\right) \right) = E_0 \cos \left( \omega t - kz \right)$
- $k = \cfrac{\omega}{v} = \omega \sqrt{\mu \varepsilon}$
- $\lambda = \cfrac{2 \pi}{k} = \cfrac{2 \pi}{\omega \sqrt{\varepsilon \mu}}$
- ${\vect{E}_1 = \vect{E}_{x} = \left(E_1 \vect{i}_{x} + 0 \vect{i}_{y} \right)e^{ - jkz}}$
- ${\vect{E}_2 = \vect{E}_{y} = \left(0 \vect{i}_{x} + E_2 \vect{i}_{y} \right)e^{ - jkz}}$
- ${e_{ x}\left(z,t\right) = E_1 \cos\left( Ï‰ t - kz \right)}$
- ${e_{y}\left(z,t\right) = E_2 \cos \left( \omega t - kz + \psi \right)}$
- ${e_{x}\left(0,t\right) = E_1 \cos{\left( \omega t\right)}}$
- ${e_{y}\left(0,t\right) = E_2 \cos{\left( \omega t + \psi\right)}}$
- $e_{x}\left(0,t\right) = E \cos{\left( \omega t\right)}$
- ${e_{y}\left(0,t\right) = E \cos{\left( \omega t \mp \cfrac{\pi}{2}\right)} = \pm E \sin{\left( \omega t\right)}}$
- ${e_{x}\left(z,0\right)} = {E \cos \left( - kz \right) = E \cos\left(kz\right)}$
- ${e_{y}\left(z,0\right)} = {E \cos \left( - kz \pm \cfrac{\pi}{2} \right) = \pm E \sin \left(kz \right)}$
- $\vect{E} =E_{y0}e^{ - jkz} \vect{i}_y$
- $\eta \vect{H} = - E_{y0}e^{ - jkz} \vect{i}_{x}$
- $\begin{aligned} P&=\int\vect{P}\cdot\opn{d}\vect{F}=\cfrac12\opn{Re} \left\{\int(\vect{E}\times\vect{H^{*}})\cdot\opn{d}\vect{F} \right\} \\ &= \cfrac{1}{2} \opn{Re} \left\{\int(E_{x}H_{y}^{*} - E_{y}H_{x}^{*}) \opn{d}F \right\} \\ &= \cfrac{w d}{2} \opn{Re} \{ - E_{y0}e^{ - j k z}( - \cfrac{E_{y0}}{\eta}e^{ + j k z}) \} = \cfrac{E_{y0}^{2}}{2 \eta}w d \end{aligned}$
- $P = \cfrac{|U|^{2}}{2Z_{\opn{PV}}}$
- $U = \int_{ - d}^{0}E_{y} \opn{d}y = E_{y0}~d$
- $P = \cfrac{|E_{y0}|^{2}d^{2}}{2Z_{\opn{PV}}}$
- $\vect{\nabla}\times\vec{E}=-j\omega\mu\vect{H}$
- $\vect{\nabla}\times\vect{H}=\sigma\vec{E}+j\omega\varepsilon\vect{E}$
- $\delta = \varepsilon - j\cfrac{\sigma}{\omega} = \varepsilon(1 - j s)$
- $s = \cfrac{1}{Q} = \tan \theta = \cfrac{\sigma}{\varepsilon \omega}$
- $\eta^{2} = \cfrac{\mu}{\delta} = \cfrac{\mu}{\varepsilon} \cfrac{1}{1 - j s}$
- $\eta = \mathbb{R} + j \mathbb{X} = \eta_{\opn{E}} \cfrac{1}{\sqrt{1 - j s}}$
- $j k_{z} = j \omega \sqrt{\mu \delta} = j \omega \sqrt{\mu \varepsilon} \sqrt{1 - j s} = \gamma = \alpha + j \beta$
- $j k_{z} = j k_{\opn{E}} \sqrt{1 - j s}$
- $\mathbb{R} = \eta_{\opn{E}} \sqrt{\cfrac{\sqrt{1 + s^{2}} + 1}{2(1 + s^{2})}} \qquad \mathbb{X} = \eta_{\opn{E}} \sqrt{\cfrac{\sqrt{1 + s^{2}} - 1}{2(1 + s^{2})}}$
-
- $\alpha = k_{\opn{E}} \sqrt{\cfrac{\sqrt{1 + s^{2}} - 1}{2}} \qquad \beta = k_{\opn{E}} \sqrt{\cfrac{\sqrt{1 + s^{2}} + 1}{2}}$
- $\eta\approx\eta_{\mathrm{E}}\left(1+j\frac{s}{2}\right)\qquad j k_{z}\approx k_{\mathrm{E}}\left(\frac{s}{2}+j\right)$
- $\eta \approx \eta_{\opn{E}} \cfrac{1 + j}{\sqrt{2s}} \qquad j k_{z} \approx k_{\opn{E}} \sqrt{\cfrac{s}{2}}\left(1 + j\right)$
- $d = \cfrac{1}{\alpha} \approx \cfrac{1}{k_{\opn{E}}} \sqrt{\cfrac{2}{s}} = \sqrt{\cfrac{2}{\omega \mu \sigma}}$