icon:: ðŸŽ‡
inherit-color-icon-from:: [[logseq-page-color-red]] 
template-used:: standard-page
tags:: [[wellenausbreitung]], [[uni]]

- $\vect{\nabla} \cdot \vect{S} = \opn{lim}_{\mathcal{V} \to0} \frac{1}{V} \oint_{\Sigma} \vect{S} \cdot \opn{d} \vect{F} = - \frac{\partial}{\partial t} \rho$
- $\vect{\nabla} \cdot( \vect{\nabla} \times \vect{H}) \equiv0$
- $\vect{\nabla} \times \vect{H} = \vect{S} + \frac{\partial}{\partial t} \vect{D}$
- $\vect{\nabla} \cdot \vect{S} = - \frac{\partial}{\partial t}( \vect{\nabla} \cdot \vect{D}) = - \frac{\partial}{\partial t} \rho$
- $\vect{\nabla} \cdot \vect{S} + \frac{\partial}{\partial t} \rho = 0$
- $\vect{\nabla} \cdot \vect{D} = \rho$
- $\vect{\nabla} \cdot \vect{B} = 0$
- $\vect{\nabla} \times \vect{E} =  - \frac{\partial}{\partial t} \vect{B}$
- $\vect{\nabla} \times \vect{H} = \vect{S} + \frac{\partial}{\partial t} \vect{D}$
- $\int_{\Sigma} \vect{D} \cdot \opn{d} \vect{F} = \int_{\tau} \rho \opn{d}V$
- $\int_{\Sigma} \vect{B} \cdot \opn{d} \vect{F} = 0$
- $\oint \vect{E} \cdot \opn{d} \vect{l} =  - \frac{\partial}{\partial t} \int_{\Sigma} \vect{B} \cdot \opn{d} \vect{F}$
- $\oint \vect{H} \cdot \opn{d} \vect{l} =  \int_{\Sigma} \vect{S} \cdot \opn{d} \vect{F} + \frac{\partial}{\partial t} \int_{\Sigma} \vect{D} \cdot \opn{d} \vect{F}$
- $\vect{F} = q \left( \vect{E} + \vect{v} \times \vect{B} \right)$
- $\vect{S} = \sigma \vect{E}$
- $\vect{S} = \rho \vect{v}$
- $\vect{D} = \varepsilon \vect{E} = \varepsilon_{r} \varepsilon_{0} \vect{E}$
- $\vect{B} = \mu \vect{H} = \mu_{r} \mu_{0} \vect{H}$
- $\frac{\partial}{\partial t} \rho( \vect{r},t) + \frac{\sigma}{\varepsilon} \rho( \vect{r},t) = 0$
- $\rho( \vect{r},t) = \rho_{0}( \vect{r})e^{ - \frac{\sigma}{\varepsilon}t}$
- $\tau_{\opn{D}} = \frac{\varepsilon}{\sigma}$
- $\vect{\nabla} \cdot \vect{E} = 0$
- $\vect{E}(x,y,z,t) = \vect{E}( \vect{r},t) = \opn{Re} \{\vect{E}( \vect{r})e^{j \omega t} \} = \frac{1}{2} \left( \vect{E}( \vect{r})e^{j \omega t} + \vect{E^{*}}( \vect{r})e^{ - j \omega t} \right)$
- $\vect{\nabla} \times \vect{H} = \vect{S} + j \omega \vect{D} = \sigma \vect{E} + j \omega \varepsilon \vect{E} = j \omega \delta \vect{E}$
- $\delta = \varepsilon + \frac{\sigma}{j \omega} = \varepsilon - j \frac{\sigma}{\omega}$
- $\tan \theta = \frac{\varepsilon^{\prime \prime}}{\varepsilon^{\prime}} = \frac{\sigma}{\omega \varepsilon}$
- $\vect{\nabla} \cdot \vect{E} = 0$
- $\vect{\nabla} \cdot \vect{H} = 0$
- $\vect{\nabla} \times \vect{E} = - j \omega \mu \vect{H}$
- $\vect{\nabla} \times \vect{H} = j \omega \delta \vect{E}$
- $\vect{P}(t) = \vect{E}(t) \times \vect{H}(t)$
- $\vect{\nabla}\cdot\vect{P}(t)=-\sigma\underbrace{{E}(t)\cdot{E}(t)}_{\vect{E^2}(t)}-\frac{\partial}{\partial t}\left(\frac{\varepsilon}{2} \underbrace{{E}(t)\cdot{E}(t)}_{\vect{E^2}(t)}+\frac{\mu}{2} \underbrace{\vect{H}(t)\cdot\vect{H}(t)}_{\vect{H^2}(t)}\right)$
  id:: 672cec6d-e05d-4a9c-9201-9036191aa824
- $w_{\opn{e}}(t) = \frac{\varepsilon}{2} \vect{E^2}(t)$
- $w_{\opn{m}}(t) = \frac{\mu}{2} \vect{H}^{2}(t)$
- $\int_{\mathcal{V}} \vect{\nabla} \cdot \vect{P}(t) \opn{d}V = \oint_{\Sigma} \vect{P}(t) \cdot \opn{d} \vect{F}$
- $- \frac{\partial}{\partial t} \int_{\mathcal{V}} \left(w_{\opn{e}}(t) + w_{\opn{m}}(t) \right) \opn{d}V = \oint_{\Sigma} \vect{P}(t) \cdot \opn{d} \vect{F} + \int_{\mathcal{V}}p_{\opn{v}}(t) \opn{d}V$
- $\vect{E}( \vect{r},t) = \frac{1}{2} \left( \vect{E}( \vect{r}) \mathit{e}^{j \omega t} + \vect{E}^{*}( \vect{r}) \mathit{e}^{ - j \omega t} \right)$
- $\vect{E}(t) \cdot \vect{E}(t) = \frac{1}{4} \left( \vect{E}( \vect{r}) \cdot \vect{E}( \vect{r})e^{2j \omega t} + 2 \vect{E}( \vect{r}) \cdot \vect{E}^{*}( \vect{r}) + \vect{E}^{*}( \vect{r}) \cdot \vect{E}^{*}( \vect{r})e^{ - 2j \omega t} \right)$
- $\overrightarrow{E}(t) \cdot \overrightarrow{E}(t) = \frac{1}{2}| \overrightarrow{E}(t)|^{2}$
- $\overline{{w_{\opn{e}}(t)}} = w_{\opn{e}} = \frac{\varepsilon}{4}| \vect{E}(t)|^{2}$
- $\overline{{w_{\opn{m}}(t)}} = w_{\opn{m}} = \frac{\mu}{4}| \vect{H}(t)|^{2}$
- $\overline{{p_{\opn{v}}(t)}} = p_{\opn{v}} = \frac{\sigma}{2}| \vect{E}(t)|^{2}$
- $\vect{T} = \frac{1}{2} \vect{E} \times \vect{H}^{*} = \vect{T}_{\opn{w}} + j \vect{T}_{\opn{b}}$
- ${{\oint \vect{E} \cdot \opn{d} \vect{l}^{\prime} = }} { E_{t1} \Delta l + E_{n1} \Delta x + E_{n2} \Delta x - E_{t2} \Delta l - E_{n2} \Delta x - E_{n1} \Delta x}$
- $= { (E_{t1} - E_{t2}) \Delta l - 0E_{n1} + 0E_{n2} = - \frac{\partial}{\partial t} \int_{F} \vect{B} \cdot \opn{d} \vect{F} = 0}$
- $E_{t1} = E_{t2}$
- $H_{t1} = H_{t2}$
- $\int \vect{D} \cdot \opn{d} \vect{F} = (D_{n1} - D_{n2}) \Delta F = \rho_{\opn{S}} \Delta F$
- $D_{n1} - D_{n2} = \rho_{\opn{S}} \quad \to \quad \varepsilon_{1}E_{n1} - \varepsilon_{2}E_{n2} = \rho_{\opn{S}}$
- $B_{n1} = B_{n2} \to \mu_{1} H_{n1} = \mu_{2}H_{n2}$
- $\vect{n} \cdot \vect{D}_{1} = \rho_{\opn{S}}$
- $\vect{n} \cdot \vect{B}_{1} = 0$
- $\vect{n} \times \vect{E}_{1} = \vect{0}$
- $\vect{n} \times \vect{H}_{1} = \vect{K}$
- $\vect{n} \cdot( \vect{D}_{1} - \vect{D}_{2}) = \rho_{8}$
- $\vect{n} \cdot( \vect{B}_{1} - \vect{B}_{2}) = 0$
- $\vect{n} \times( \vect{E}_{1} - \vect{E}_{2}) = \vect{0}$
- $\vect{n} \times( \vect{H}_{1} - \vect{H}_{2}) = \vect{K}$
- $\nabla^{2} \vect{E} - \mu \varepsilon \frac{\partial^{2}}{\partial t^{2}} \vect{E} - \mu \sigma \frac{\partial}{\partial t} \vect{E} = 0$
- $\nabla^{2} \vect{E} + ( \omega^{2} \mu \varepsilon - j \omega \mu \sigma) \vect{E} = 0$
- $\nabla^{2} \vect{E} + \omega^{2} \mu \delta \vect{E} = 0$
- $\nabla^{2} = \frac{\partial^{2}}{\partial x^{2}} + \frac{\partial^{2}}{\partial y^{2}} + \frac{\partial^{2}}{\partial z^{2}}$
- $k = \omega \sqrt{\mu \delta}$
- $\Psi(x,y,z) = X(x)Y(y)Z(z)$
- $\frac{1}{X(x)} \frac{\partial^{2}}{\partial x^{2}}X(x) + \frac{1}{Y(y)} \frac{\partial^{2}}{\partial y^{2}}Y(y) + \frac{1}{Z(z)} \frac{\partial^{2}}{\partial z^{2}}Z(z) + \underbrace{k^{2}}_{\opn{const.}} = 0$
- $\frac{1}{X(x)} \frac{\partial^{2}}{\partial x^{2}}X(x) = - k_{x}^{2}$
- $k_{x}^{2} + k_{y}^{2} + k_{z}^{2} = k^{2} = \omega^{2} \mu \delta$
- $\frac{\partial^{2}}{\partial x^{2}}X(x) + k_{x}^{2}X(x) = 0$
- $\frac{\partial}{\partial y}H_{z} - \frac{\partial}{\partial z}H_{y} = j \omega \delta E_{x}$
- $\frac{\partial}{\partial z}H_{x} - \frac{\partial}{\partial x}H_{z} = j \omega \delta E_{y}$
- $\frac{\partial}{\partial x}H_{y} - \frac{\partial}{\partial y}H_{x} = j \omega \delta E_{z}$
- $\frac{\partial}{\partial y}E_{z} - \frac{\partial}{\partial z}E_{y} = - j \omega \mu H_{x}$
- $\frac{\partial}{\partial z}E_{x} - \frac{\partial}{\partial x}E_{z} = - j \omega \mu H_{y}$
- $\frac{\partial}{\partial x}E_{y} - \frac{\partial}{\partial y}E_{x} = - j \omega \mu H_{z}$
- $E_{x} = \frac{ - j}{\kappa^{2}} \left(k_{z} \frac{\partial}{\partial x}E_{z} + \omega \mu \frac{\partial}{\partial y}H_{z} \right)$
- $E_{y} = \frac{ - j}{\kappa^{2}} \left(k_{z} \frac{\partial}{\partial y}E_{z} - \omega \mu \frac{\partial}{\partial x}H_{z} \right)$
- $H_{x} = \frac{ - j}{\kappa^{2}} \left(k_{z} \frac{\partial}{\partial x}H_{z} - \omega \delta \frac{\partial}{\partial y}E_{z} \right)$
- $H_{y} = \frac{ - j}{\kappa^{2}} \left( k_{z} \frac{\partial}{\partial y} H_{z} + \omega \delta \frac{\partial}{\partial x} E_{z} \right)$